Rename fmap_foo to env_foo

Launchbury/Env.thy
@@ -4,7 +4,12 @@ begin
 
 default_sort type
 
-subsubsection {* The type of finite maps *}
+text {*
+Our type for environments is a function with a pcpo as the co-domain; this theory collects
+related definitions.
+*}
+
+subsubsection {* The domain of a pcpo-valued function *}
 
 definition fdom :: "('key \<Rightarrow> 'value::pcpo) \<Rightarrow> 'key set" where "fdom m = {x. m x \<noteq> \<bottom>}"
 
@@ -27,109 +32,109 @@ declare fun_upd_same[simp] fun_upd_other[simp]
 
 subsubsection {* Restriction *}
 
-definition fmap_restr :: "'a set \<Rightarrow> ('a \<Rightarrow> 'b::pcpo) \<Rightarrow> ('a \<Rightarrow> 'b)"
-  where "fmap_restr S m = (\<lambda> x. if x \<in> S then m x else \<bottom>)"
+definition env_restr :: "'a set \<Rightarrow> ('a \<Rightarrow> 'b::pcpo) \<Rightarrow> ('a \<Rightarrow> 'b)"
+  where "env_restr S m = (\<lambda> x. if x \<in> S then m x else \<bottom>)"
 
-abbreviation fmap_restr_rev  (infixl "f|`"  110) where "fmap_restr_rev m S \<equiv> fmap_restr S m"
+abbreviation env_restr_rev  (infixl "f|`"  110) where "env_restr_rev m S \<equiv> env_restr S m"
 
-notation (latex output) fmap_restr_rev ("_|\<^bsub>_\<^esub>")
+notation (latex output) env_restr_rev ("_|\<^bsub>_\<^esub>")
 
-lemma fmap_restr_empty[simp]: "fdom m \<inter> S = {} \<Longrightarrow> m f|` S = \<bottom>"
-  by (fastforce simp add: fdom_def fmap_restr_def)
+lemma env_restr_empty[simp]: "fdom m \<inter> S = {} \<Longrightarrow> m f|` S = \<bottom>"
+  by (fastforce simp add: fdom_def env_restr_def)
 
-lemma lookup_fmap_restr[simp]: "x \<in> S \<Longrightarrow> (fmap_restr S m) x = m x"
-  by (fastforce simp add: fmap_restr_def)
+lemma lookup_env_restr[simp]: "x \<in> S \<Longrightarrow> (env_restr S m) x = m x"
+  by (fastforce simp add: env_restr_def)
 
-lemma lookup_fmap_restr_not_there[simp]: "x \<notin> S \<Longrightarrow> (fmap_restr S m) x = \<bottom>"
-  by (fastforce simp add: fmap_restr_def)
+lemma lookup_env_restr_not_there[simp]: "x \<notin> S \<Longrightarrow> (env_restr S m) x = \<bottom>"
+  by (fastforce simp add: env_restr_def)
 
-lemma lookup_fmap_restr_eq: "(m f|` S) x = (if x \<in> S then m x else \<bottom>)"
+lemma lookup_env_restr_eq: "(m f|` S) x = (if x \<in> S then m x else \<bottom>)"
   by simp
 
-lemma fmap_restr_cong: "fdom m \<inter> S1 = fdom m \<inter> S2 \<Longrightarrow> m f|` S1 = m f|` S2"
+lemma env_restr_cong: "fdom m \<inter> S1 = fdom m \<inter> S2 \<Longrightarrow> m f|` S1 = m f|` S2"
   apply (rule ext)
-  apply (simp add: lookup_fmap_restr_eq)
+  apply (simp add: lookup_env_restr_eq)
   by (metis Int_iff lookup_not_fdom)
 
-lemma fmap_restr_fmap_restr[simp]:
+lemma env_restr_env_restr[simp]:
  "x f|` d2 f|` d1 = x f|` (d1 \<inter> d2)"
-  by (fastforce simp add: fmap_restr_def)
+  by (fastforce simp add: env_restr_def)
 
-lemma fmap_restr_fmap_restr_subset:
+lemma env_restr_env_restr_subset:
  "d1 \<subseteq> d2 \<Longrightarrow> x f|` d2 f|` d1 = x f|` d1"
- by (metis Int_absorb2 fmap_restr_fmap_restr)
+ by (metis Int_absorb2 env_restr_env_restr)
 
-lemma fmap_restr_useless: "fdom m \<subseteq> S \<Longrightarrow> m f|` S = m"
-  by (rule ext) (auto simp add: lookup_fmap_restr_eq dest!: set_mp)
+lemma env_restr_useless: "fdom m \<subseteq> S \<Longrightarrow> m f|` S = m"
+  by (rule ext) (auto simp add: lookup_env_restr_eq dest!: set_mp)
 
-lemma fmap_restr_UNIV[simp]: "m f|` UNIV = m"
-  by (rule fmap_restr_useless) simp
+lemma env_restr_UNIV[simp]: "m f|` UNIV = m"
+  by (rule env_restr_useless) simp
 
-lemma fmap_restr_fun_upd[simp]: "x \<in> S \<Longrightarrow> m1(x := v) f|` S = (m1 f|` S)(x := v)"
+lemma env_restr_fun_upd[simp]: "x \<in> S \<Longrightarrow> m1(x := v) f|` S = (m1 f|` S)(x := v)"
   apply (rule ext)
   apply (case_tac "xa = x")
-  apply (auto simp add: lookup_fmap_restr_eq)
+  apply (auto simp add: lookup_env_restr_eq)
   done
 
-lemma fmap_restr_fun_upd_other[simp]: "x \<notin> S \<Longrightarrow> m1(x := v) f|` S = m1 f|` S"
+lemma env_restr_fun_upd_other[simp]: "x \<notin> S \<Longrightarrow> m1(x := v) f|` S = m1 f|` S"
   apply (rule ext)
   apply (case_tac "xa = x")
-  apply (auto simp add: lookup_fmap_restr_eq)
+  apply (auto simp add: lookup_env_restr_eq)
   done
 
-lemma fmap_restr_eq_subset:
+lemma env_restr_eq_subset:
   assumes "S \<subseteq> S'"
   and "m1 f|` S' = m2 f|` S'"
   shows "m1 f|` S = m2 f|` S"
 using assms
-by (metis fmap_restr_fmap_restr le_iff_inf)
+by (metis env_restr_env_restr le_iff_inf)
 
 subsubsection {* Deleting *}
 
-definition fmap_delete :: "'a \<Rightarrow> ('a \<Rightarrow> 'b) \<Rightarrow> ('a \<Rightarrow> 'b::pcpo)"
-  where "fmap_delete x m = m(x := \<bottom>)"
+definition env_delete :: "'a \<Rightarrow> ('a \<Rightarrow> 'b) \<Rightarrow> ('a \<Rightarrow> 'b::pcpo)"
+  where "env_delete x m = m(x := \<bottom>)"
 
-lemma lookup_fmap_delete[simp]:
-  "x' \<noteq> x \<Longrightarrow> fmap_delete x m x' = m x'"
-  by (simp add: fmap_delete_def)
+lemma lookup_env_delete[simp]:
+  "x' \<noteq> x \<Longrightarrow> env_delete x m x' = m x'"
+  by (simp add: env_delete_def)
 
-lemma lookup_fmap_delete_None[simp]:
-  "fmap_delete x m x = \<bottom>"
-  by (simp add: fmap_delete_def)
+lemma lookup_env_delete_None[simp]:
+  "env_delete x m x = \<bottom>"
+  by (simp add: env_delete_def)
 
-lemma fdom_fmap_delete[simp]:
-  "fdom (fmap_delete x m) = fdom m - {x}"
-  by (auto simp add: fmap_delete_def fdom_def)
+lemma fdom_env_delete[simp]:
+  "fdom (env_delete x m) = fdom m - {x}"
+  by (auto simp add: env_delete_def fdom_def)
 
-lemma fdom_fmap_delete_subset:
-  "fdom (fmap_delete x m) \<subseteq> fdom m" by auto
+lemma fdom_env_delete_subset:
+  "fdom (env_delete x m) \<subseteq> fdom m" by auto
 
-lemma fmap_delete_fun_upd[simp]:
-  "fmap_delete x (m(x := v)) = fmap_delete x m"
-  by (auto simp add: fmap_delete_def)
+lemma env_delete_fun_upd[simp]:
+  "env_delete x (m(x := v)) = env_delete x m"
+  by (auto simp add: env_delete_def)
 
-lemma fmap_delete_fun_upd2[simp]:
-  "(fmap_delete x m)(x := v) = m(x := v)"
-  by (auto simp add: fmap_delete_def)
+lemma env_delete_fun_upd2[simp]:
+  "(env_delete x m)(x := v) = m(x := v)"
+  by (auto simp add: env_delete_def)
 
-lemma fmap_delete_fun_upd3[simp]:
-  "x \<noteq> y \<Longrightarrow> fmap_delete x (m(y := v)) = (fmap_delete x m)(y := v)"
-  by (auto simp add: fmap_delete_def)
+lemma env_delete_fun_upd3[simp]:
+  "x \<noteq> y \<Longrightarrow> env_delete x (m(y := v)) = (env_delete x m)(y := v)"
+  by (auto simp add: env_delete_def)
 
-lemma fmap_delete_noop[simp]:
-  "x \<notin> fdom m \<Longrightarrow> fmap_delete x m = m"
-  by (auto simp add: fmap_delete_def fdom_def)
+lemma env_delete_noop[simp]:
+  "x \<notin> fdom m \<Longrightarrow> env_delete x m = m"
+  by (auto simp add: env_delete_def fdom_def)
 
-lemma fun_upd_fmap_delete[simp]: "x \<in> fdom \<Gamma> \<Longrightarrow> (fmap_delete x \<Gamma>)(x := \<Gamma> x) = \<Gamma>"
+lemma fun_upd_env_delete[simp]: "x \<in> fdom \<Gamma> \<Longrightarrow> (env_delete x \<Gamma>)(x := \<Gamma> x) = \<Gamma>"
   by (auto)
 
-lemma fmap_restr_fmap_delete_other[simp]: "x \<notin> S \<Longrightarrow> fmap_delete x m f|` S = m f|` S"
+lemma env_restr_env_delete_other[simp]: "x \<notin> S \<Longrightarrow> env_delete x m f|` S = m f|` S"
   apply (rule ext)
-  apply (auto simp add: lookup_fmap_restr_eq)
-  by (metis lookup_fmap_delete)
+  apply (auto simp add: lookup_env_restr_eq)
+  by (metis lookup_env_delete)
 
-lemma fmap_delete_restr: "fmap_delete x m = m f|` (-{x})"
-  by (auto simp add: lookup_fmap_restr_eq)
+lemma env_delete_restr: "env_delete x m = m f|` (-{x})"
+  by (auto simp add: lookup_env_restr_eq)
 
 subsubsection {* Merging of two functions *}
 
@@ -139,11 +144,10 @@ We'd like to have some nice syntax for @{term "override_on"}.
 
 abbreviation override_on_syn ("_ ++\<^bsub>_\<^esub> _" [100, 0, 100] 100) where "f1 ++\<^bsub>S\<^esub> f2 \<equiv> override_on f1 f2 S"
 
-lemma override_on_fempty[simp]: "\<bottom> ++\<^bsub>S\<^esub> m = m f|` S" 
-  by (auto simp add: override_on_def fmap_restr_def)
-
-lemma override_on_fempty2[simp]: "m ++\<^bsub>S\<^esub> \<bottom> = m f|` (-S)" 
-  by (auto simp add: override_on_def fmap_restr_def)
+lemma override_on_bot[simp]:
+  "\<bottom> ++\<^bsub>S\<^esub> m = m f|` S" 
+  "m ++\<^bsub>S\<^esub> \<bottom> = m f|` (-S)" 
+  by (auto simp add: override_on_def env_restr_def)
 
 lemma fdom_override_on[simp]: "fdom (m1 ++\<^bsub>S\<^esub> m2) = (fdom m1 - S) \<union> (fdom m2 \<inter> S)"
   by (auto simp add: override_on_def fdom_def)
@@ -159,10 +163,10 @@ lemma override_on_upd:
   "x \<in> S \<Longrightarrow> \<rho> ++\<^bsub>S\<^esub> (\<rho>'(x := z)) = (\<rho> ++\<^bsub>S - {x}\<^esub> \<rho>')(x := z)"
   by (auto simp add: override_on_def  fdom_def)
 
-lemma fmap_restr_add: "(m1 ++\<^bsub>S2\<^esub> m2) f|` S = m1 f|` S ++\<^bsub>S2\<^esub> m2 f|` S"
-  by (auto simp add: override_on_def  fdom_def fmap_restr_def)
+lemma env_restr_add: "(m1 ++\<^bsub>S2\<^esub> m2) f|` S = m1 f|` S ++\<^bsub>S2\<^esub> m2 f|` S"
+  by (auto simp add: override_on_def  fdom_def env_restr_def)
 
-lemma fmap_delete_add: "fmap_delete x (m1 ++\<^bsub>S\<^esub> m2) = fmap_delete x m1 ++\<^bsub>S - {x}\<^esub> fmap_delete x m2"
-  by (auto simp add: override_on_def  fdom_def fmap_restr_def fmap_delete_def)
+lemma env_delete_add: "env_delete x (m1 ++\<^bsub>S\<^esub> m2) = env_delete x m1 ++\<^bsub>S - {x}\<^esub> env_delete x m2"
+  by (auto simp add: override_on_def  fdom_def env_restr_def env_delete_def)
 
 end
