Launchbury/Env-HOLCF.thy
@@ -43,12 +43,12 @@ lemma fun_upd_belowI:
   apply auto
   done
 
-lemma fun_upd_below_fmap_deleteI:
-  assumes "fmap_delete x \<rho> \<sqsubseteq> fmap_delete x \<rho>'" 
+lemma fun_upd_below_env_deleteI:
+  assumes "env_delete x \<rho> \<sqsubseteq> env_delete x \<rho>'" 
   assumes "y \<sqsubseteq> \<rho>' x"
   shows  "\<rho>(x := y) \<sqsubseteq> \<rho>'"
   using assms
-  apply (auto intro!: fun_upd_belowI   simp add: fmap_delete_def)
+  apply (auto intro!: fun_upd_belowI   simp add: env_delete_def)
   by (metis fun_belowD fun_upd_other)
 
 lemma fun_upd_belowI2:
@@ -58,65 +58,65 @@ lemma fun_upd_belowI2:
   apply (rule fun_belowI)
   using assms by auto
 
-lemma fmap_restr_belowI:
+lemma env_restr_belowI:
   assumes  "\<And> x. x \<in> S \<Longrightarrow> (m1 f|` S) x \<sqsubseteq> (m2 f|` S) x"
   shows "m1 f|` S \<sqsubseteq> m2 f|` S"
   apply (rule fun_belowI)
-  by (metis assms below_bottom_iff lookup_fmap_restr_not_there)
+  by (metis assms below_bottom_iff lookup_env_restr_not_there)
 
-lemma fmap_restr_below_itself:
+lemma env_restr_below_itself:
   shows "m f|` S \<sqsubseteq> m"
   apply (rule fun_belowI)
   apply (case_tac "x \<in> S")
   apply auto
   done  
 
-lemma fmap_restr_cont:  "cont (fmap_restr S)"
+lemma env_restr_cont:  "cont (env_restr S)"
   apply (rule cont2cont_lambda)
   apply (case_tac "y \<in> S")
   apply (auto simp add: assms)
   done
 
-lemma fmap_restr_belowD:
+lemma env_restr_belowD:
   assumes "m1 f|` S \<sqsubseteq> m2 f|` S"
   assumes "x \<in> S"
   shows "m1 x \<sqsubseteq> m2 x"
   using fun_belowD[OF assms(1), where x = x] assms(2) by simp
 
-lemma fmap_restr_eqD:
+lemma env_restr_eqD:
   assumes "m1 f|` S = m2 f|` S"
   assumes "x \<in> S"
   shows "m1 x = m2  x"
-  by (metis assms(1) assms(2) lookup_fmap_restr)
+  by (metis assms(1) assms(2) lookup_env_restr)
 
-lemma fmap_restr_below_subset:
+lemma env_restr_below_subset:
   assumes "S \<subseteq> S'"
   and "m1 f|` S' \<sqsubseteq> m2 f|` S'"
   shows "m1 f|` S \<sqsubseteq> m2 f|` S"
 using assms
-by (auto intro!: fmap_restr_belowI dest: fmap_restr_belowD)
+by (auto intro!: env_restr_belowI dest: env_restr_belowD)
 
 lemma  override_on_below_restrI:
   assumes " x f|` (-S) \<sqsubseteq> z f|` (-S)"
   and "y f|` S \<sqsubseteq> z f|` S"
   shows  "x ++\<^bsub>S\<^esub> y \<sqsubseteq> z"
 using assms
-by (auto intro: override_on_belowI dest:fmap_restr_belowD)
+by (auto intro: override_on_belowI dest:env_restr_belowD)
 
 lemma  fmap_below_add_restrI:
   assumes "x f|` (-S) \<sqsubseteq> y f|` (-S)"
   and     "x f|` S \<sqsubseteq> z f|` S"
   shows  "x \<sqsubseteq> y ++\<^bsub>S\<^esub> z"
 using assms
-by (auto intro!: fun_belowI dest:fmap_restr_belowD simp add: lookup_override_on_eq)
+by (auto intro!: fun_belowI dest:env_restr_belowD simp add: lookup_override_on_eq)
 
-lemmas fmap_restr_cont2cont[simp,cont2cont] = cont_compose[OF fmap_restr_cont]
+lemmas env_restr_cont2cont[simp,cont2cont] = cont_compose[OF env_restr_cont]
 
-lemma fmap_delete_cont:  "cont (fmap_delete x)"
+lemma env_delete_cont:  "cont (env_delete x)"
   apply (rule cont2cont_lambda)
   apply (case_tac "y = x")
   apply (auto simp add: assms)
   done
-lemmas fmap_delete_cont2cont[simp,cont2cont] = cont_compose[OF fmap_delete_cont]
+lemmas env_delete_cont2cont[simp,cont2cont] = cont_compose[OF env_delete_cont]
 
 end
