Launchbury/Env-Nominal.thy
@@ -16,15 +16,15 @@ lemma mem_fdom_perm[simp]:
   shows "xa \<in> fdom (p \<bullet> \<rho>) \<longleftrightarrow> - p \<bullet> xa \<in> fdom \<rho>" 
   by (metis (mono_tags) fdom_perm_rev mem_Collect_eq permute_set_eq)
 
-lemma fmap_restr_eqvt[eqvt]:
+lemma env_restr_eqvt[eqvt]:
   fixes m :: "'a::pt \<Rightarrow> 'b::{cont_pt,pcpo}"
   shows "\<pi> \<bullet> m f|` d = (\<pi> \<bullet> m) f|` (\<pi> \<bullet> d)"
-  by (auto simp add: fmap_restr_def)
+  by (auto simp add: env_restr_def)
 
-lemma fmap_delete_eqvt[eqvt]:
+lemma env_delete_eqvt[eqvt]:
   fixes m :: "'a::pt \<Rightarrow> 'b::{cont_pt,pcpo}"
-  shows "\<pi> \<bullet> fmap_delete x m = fmap_delete (\<pi> \<bullet> x) (\<pi> \<bullet> m)"
-  by (auto simp add: fmap_delete_def)
+  shows "\<pi> \<bullet> env_delete x m = env_delete (\<pi> \<bullet> x) (\<pi> \<bullet> m)"
+  by (auto simp add: env_delete_def)
 
 lemma override_on_eqvt[eqvt]:
   fixes m1 m2 :: "'a::pt \<Rightarrow> 'b::{cont_pt,pcpo}"
@@ -33,7 +33,7 @@ lemma override_on_eqvt[eqvt]:
 
 subsubsection {* Permutation and restriction *}
 
-lemma fmap_restr_perm:
+lemma env_restr_perm:
   fixes \<rho> :: "'a::at_base \<Rightarrow> 'b::{pcpo_pt,pure}"
   assumes "supp p \<sharp>* S" and [simp]: "finite S"
   shows "(p \<bullet> \<rho>) f|` S = \<rho> f|` S"
@@ -48,14 +48,14 @@ apply (subst perm_supp_eq)
 apply (auto simp add:perm_supp_eq supp_minus_perm fresh_star_def fresh_def supp_set_elem_finite)
 done
 
-lemma fmap_restr_flip:
+lemma env_restr_flip:
   fixes \<rho> :: "'a::at \<Rightarrow> 'b::{pcpo_pt,pure}"
   assumes "x \<notin> S" and "x' \<notin> S"
   shows "((x' \<leftrightarrow> x) \<bullet> \<rho>) f|` S = \<rho> f|` S"
   using assms
   apply -
   apply rule
-  apply (auto  simp add: permute_flip_at fmap_restr_def split:if_splits)
+  apply (auto  simp add: permute_flip_at env_restr_def split:if_splits)
   by (metis eqvt_lambda flip_at_base_simps(3) minus_flip permute_pure unpermute_def)
 
 end
